updates

code/experimental/ed25519/Hacl.Impl.Ed25519.Sign.fst
@@ -1,5 +1,7 @@
 module Hacl.Impl.Ed25519.Sign
 
+
+open FStar.Mul
 open FStar.Buffer
 open FStar.UInt32
 
@@ -10,89 +12,7 @@ let hint8_p = buffer Hacl.UInt8.t
 let op_String_Access h b = Hacl.Spec.Endianness.reveal_sbytes (as_seq h b)
 
 
-#reset-options "--max_fuel 0 --z3rlimit 20"
-
-[@ "substitute"]
-private
-val point_mul_compress:
-  out:hint8_p{length out = 32} ->
-  s:hint8_p{length s = 32} ->
-  p:point ->
-  Stack unit
-    (requires (fun h -> live h out /\ live h s /\ live h p /\ point_inv h p))
-    (ensures (fun h0 _ h1 -> live h1 out /\ live h0 s /\ live h0 p /\ modifies_1 out h0 h1 /\
-      h1.[out] == Spec.Ed25519.(point_compress (point_mul h0.[s] (as_point h0 p)))))
-
-#reset-options "--max_fuel 0 --z3rlimit 200"
-
-let point_mul_compress out s p =
-  push_frame();
-  let tmp:point = Buffer.create 0uL 20ul in
-  Hacl.Impl.Ed25519.Ladder.point_mul tmp s p;
-  Hacl.Impl.Ed25519.PointCompress.point_compress out tmp;
-  pop_frame()
-
-
-#reset-options "--max_fuel 0 --z3rlimit 20"
-
-[@ "substitute"]
-private
-val copy_bytes:
-  output:hint8_p ->
-  input:hint8_p{disjoint input output} ->
-  len:UInt32.t{length output = UInt32.v len /\ length input = UInt32.v len} ->
-  Stack unit
-    (requires (fun h -> live h output /\ live h input))
-    (ensures (fun h0 _ h1 -> live h0 input /\ live h1 output /\ modifies_1 output h0 h1
-      /\ as_seq h1 output == as_seq h0 input))
-let copy_bytes output input len =
-  let h0 = ST.get() in
-  blit input 0ul output 0ul len;
-  let h1 = ST.get() in
-  Seq.lemma_eq_intro (as_seq h0 input) (Seq.slice (as_seq h0 input) 0 (UInt32.v len));
-  Seq.lemma_eq_intro (as_seq h1 output) (Seq.slice (as_seq h1 output) 0 (UInt32.v len))
-
-
-#reset-options "--max_fuel 0 --z3rlimit 200"
-
-
-private
-val lemma_append:
-  h:HyperStack.mem ->
-  buf:hint8_p{live h buf} ->
-  len1:UInt32.t ->
-  len2:UInt32.t ->
-  len3:UInt32.t{UInt32.v len3 + UInt32.v len2 + UInt32.v len1 = length buf} ->
-  Lemma (as_seq h buf == FStar.Seq.(as_seq h (Buffer.sub buf 0ul len1) @| as_seq h (Buffer.sub buf len1 len2) @| (as_seq h (Buffer.sub buf FStar.UInt32.(len1 +^ len2) len3))))
-
-#reset-options "--max_fuel 0 --z3rlimit 200"
-
-let lemma_append h buf len1 len2 len3 =
-  let open FStar.UInt32 in
-  let b = as_seq h buf in
-  Seq.lemma_eq_intro (as_seq h (Buffer.sub buf 0ul len1)) (Seq.slice b 0 (v len1));
-  Seq.lemma_eq_intro (as_seq h (Buffer.sub buf len1 len2)) (Seq.slice b (v len1) (v len1 + v len2));
-  Seq.lemma_eq_intro (as_seq h (Buffer.sub buf FStar.UInt32.(len1 +^ len2) len3)) (Seq.slice b (v len1 + v len2) (v len1 + v len2 + v len3));
-  Seq.lemma_eq_intro b FStar.Seq.(slice b 0 (v len1) @| slice b (v len1) (v len1 + v len2) @| slice b (v len1 + v len2) (v len1 + v len2 + v len3))
-
-
-private
-val lemma_append2:
-  h:HyperStack.mem ->
-  buf:hint8_p{live h buf} ->
-  len1:UInt32.t ->
-  len2:UInt32.t{UInt32.v len1 + UInt32.v len2 = length buf} ->
-  Lemma (as_seq h buf == FStar.Seq.(as_seq h (Buffer.sub buf 0ul len1) @| as_seq h (Buffer.sub buf len1 len2)))
-
-let lemma_append2 h buf len1 len2 =
-  let open FStar.UInt32 in
-  let b = as_seq h buf in
-  Seq.lemma_eq_intro (as_seq h (Buffer.sub buf 0ul len1)) (Seq.slice b 0 (v len1));
-  Seq.lemma_eq_intro (as_seq h (Buffer.sub buf len1 len2)) (Seq.slice b (v len1) (v len1 + v len2));
-  Seq.lemma_eq_intro b FStar.Seq.(slice b 0 (v len1) @| slice b (v len1) (v len1 + v len2))
-
-
-#reset-options "--max_fuel 0 --z3rlimit 20"
+open Hacl.Impl.Ed25519.Sign.Steps
 
 [@ "substitute"]
 private
@@ -116,7 +36,7 @@ val sign__:
 #reset-options "--max_fuel 0 --z3rlimit 200"
 
 let sign__ signature secret msg len g tmp_bytes tmp_ints =
-  push_frame();
+  let tmp_bytes' = tmp_bytes in
   let tmpa = Buffer.sub tmp_ints 0ul  20ul in
   let r    = Buffer.sub tmp_ints 20ul 5ul  in
   let r'   = Buffer.sub tmp_ints 25ul 20ul in
@@ -132,44 +52,25 @@ let sign__ signature secret msg len g tmp_bytes tmp_ints =
   let rs'  = Buffer.sub tmp_bytes 160ul 32ul in
   let s'   = Buffer.sub tmp_bytes 192ul 32ul in
   let apre = Buffer.sub tmp_bytes 224ul 64ul in
-  Hacl.Impl.Ed25519.SecretExpand.secret_expand apre secret;
-  let a      = Buffer.sub apre 0ul 32ul in
-  let prefix = Buffer.sub apre 32ul 64ul in
-  point_mul_compress a'' a g;
+  
+  sign_step_1 signature secret msg len g tmp_bytes' tmp_ints;
+
   (* TODO: use an incremental version of SHA instead so as to minimize
   the copies and enable compilation with CompCert *)
-  let prefix_at_msg = Buffer.sub prefix_at_message 32ul FStar.UInt32.(32ul +^ len) in
-  let message       = Buffer.sub prefix_at_msg 32ul len in
-  let prefix'       = Buffer.sub prefix_at_msg 0ul 32ul in
-  copy_bytes prefix' prefix 32ul;
-  let h0 = ST.get() in
-  lemma_append2 h0 prefix_at_msg 32ul len;
-  Hacl.Impl.SHA512.ModQ.sha512_modq r prefix_at_msg (len+^32ul);
-  Hacl.Impl.Store56.store_56 rb r;
-  point_mul_compress rs' rb g;
-  (* Hacl.Impl.Ed25519.Ladder.point_mul r' rb g; *)
-  (* Hacl.Impl.Ed25519.PointCompress.point_compress rs' r'; *)
-  let rs_bytes = Buffer.sub prefix_at_message 0ul  32ul in
-  let a_bytes  = Buffer.sub prefix_at_message 32ul 32ul in
-  copy_bytes rs_bytes rs' 32ul;
-  copy_bytes a_bytes a'' 32ul;
-  (* blit rs'  0ul prefix_at_message 0ul 32ul; *)
-  (* blit a''  0ul prefix_at_message 32ul 32ul; *)
-  let h' = ST.get() in
-  lemma_append h' prefix_at_message 32ul 32ul len;
-  Hacl.Impl.SHA512.ModQ.sha512_modq h prefix_at_message (len+^64ul);
-  Hacl.Impl.Load56.load_32_bytes aq a;
-  Hacl.Impl.BignumQ.Mul.mul_modq ha h aq;
-  Hacl.Impl.BignumQ.Mul.add_modq s r ha;
-  Hacl.Impl.Store56.store_56 s' s;
+
+  sign_step_2 signature secret msg len g tmp_bytes' tmp_ints;
+
+  sign_step_3 signature secret msg len g tmp_bytes' tmp_ints;
+
+  sign_step_4 signature secret msg len g tmp_bytes' tmp_ints;
+
+  sign_step_5 signature secret msg len g tmp_bytes' tmp_ints;
+
   copy_bytes (Buffer.sub signature 0ul 32ul) rs' 32ul;
   copy_bytes (Buffer.sub signature 32ul 32ul) s' 32ul;
   let h'' = ST.get() in
-  lemma_append2 h'' signature 32ul 32ul;
-  admit();
-  (* blit rs' 0ul signature 0ul 32ul; *)
-  (* blit s' 0ul signature 32ul 32ul; *)
-  pop_frame()
+  (* lemma_append2 h'' signature 32ul 32ul; *)
+  ()
 
 
 #reset-options "--max_fuel 0 --z3rlimit 20"
@@ -187,18 +88,22 @@ val sign_:
       live h1 signature /\ modifies_1 signature h0 h1 /\
       h1.[signature] == Spec.Ed25519.sign h0.[secret] h0.[msg]))
 
-#reset-options "--max_fuel 0 --z3rlimit 100"
+#reset-options "--max_fuel 0 --z3rlimit 50"
 
 let sign_ signature secret msg len g =
   push_frame();
   let tmp_bytes = Buffer.create 0uy (352ul +^ len) in
   push_frame();
-  let h0 = ST.get() in  
+  let h0 = ST.get() in
   let tmp_ints  = Buffer.create 0uL 65ul in
   let msg'      = Buffer.sub tmp_bytes 64ul len in
   let h1 = ST.get() in
+  no_upd_lemma_0 h0 h1 g;
+  no_upd_lemma_0 h0 h1 msg;
   copy_bytes msg' msg len;
   let h2 = ST.get() in
+  no_upd_lemma_1 h1 h2 msg' g;
+  assert(modifies_0 h0 h2);
   sign__ signature secret msg len g tmp_bytes tmp_ints;
   let h3 = ST.get() in
   pop_frame();
@@ -209,16 +114,22 @@ val sign:
   signature:hint8_p{length signature = 64} ->
   secret:hint8_p{length secret = 32} ->
   msg:hint8_p{length msg < pow2 32 - 64} ->
-  len:UInt32.t{UInt32.v len = length msg} ->
+  len:UInt32.t{UInt32.v len = length msg /\ UInt32.v len + 352 < pow2 32} ->
   Stack unit
     (requires (fun h -> live h signature /\ live h msg /\ live h secret))
     (ensures (fun h0 _ h1 -> live h0 signature /\ live h0 msg /\ live h0 secret /\
       live h1 signature /\ modifies_1 signature h0 h1 /\
       h1.[signature] == Spec.Ed25519.sign h0.[secret] h0.[msg]))
 
+#reset-options "--max_fuel 0 --z3rlimit 20"
+
 let sign signature secret msg len =
   push_frame();
+  let h0 = ST.get() in
   let g = create 0uL 20ul in
   Hacl.Impl.Ed25519.G.make_g g;
-  sign_ signature secret msg len g;  
+  let h1 = ST.get() in
+  assume (as_point h1 g == Spec.Ed25519.g);
+  sign_ signature secret msg len g;
+  let h2 = ST.get() in
   pop_frame()
